Weidenbach_Book/IsaSAT_Lookup_Conflict.thy
@@ -1612,7 +1612,8 @@ lemma minimize_and_extract_highest_lookup_conflict_iterate_over_conflict:
     lits_D: \<open>literals_are_in_\<L>\<^sub>i\<^sub>n D\<close>
   shows
     \<open>minimize_and_extract_highest_lookup_conflict M NU D' s' \<le>
-       \<Down> ({((D, s, L'), (D', L)). (D, D') \<in> lookup_clause_rel \<and> L' = L})
+       \<Down> ({((E, s, L'), (E', L)). (E, E') \<in> lookup_clause_rel \<and> L' = L \<and> length (snd E) = length (snd D') \<and>
+               E' \<subseteq># D})
            (iterate_over_conflict K M NU' NUP D)\<close>
     (is \<open>_ \<le> \<Down> ?R _\<close>)
 proof -
@@ -2258,7 +2259,8 @@ lemma
     lits_D: \<open>literals_are_in_\<L>\<^sub>i\<^sub>n D\<close>
   shows
     \<open>minimize_and_extract_highest_lookup_conflict M NU D' s' \<le>
-       \<Down> ({((D, s, L'), (D', L)). (D, D') \<in> lookup_clause_rel \<and> L' = L})
+       \<Down> ({((E, s, L'), (E', L)). (E, E') \<in> lookup_clause_rel \<and> L' = L \<and>
+            length (snd E) = length (snd D') \<and> E' \<subseteq># D})
          (SPEC (\<lambda>(D', highest). D' \<subseteq># D \<and> NU' + NUP \<Turnstile>pm add_mset K D' \<and>
             highest_lit M D' highest))\<close>
 proof -
